spec verifies (no interesting properties yet)

tla-tree/CrashSafeTree.dfy
@@ -2,6 +2,7 @@ include "KVTypes.dfy"
 include "Disk.dfy"
 
 module TreeDisk refines Disk {
+//export reveals Child, Node, Sector
 import opened KVTypes
 
 // Every sector is either
@@ -10,12 +11,11 @@ import opened KVTypes
 // subject to owner agreement; visited on fsck), or 
 // * Cold (in a persistent free list of cold sectors).
 datatype Child = Value(datum:Datum) | Pointer(lba:LBA) | Empty
-// TODO consider breaking Node into a separate datatype so that path manipulations,
-// which never talk about non-Nodes, can skip the .Node? tests.
+datatype Node = Node(parent:LBA, pivots:seq<Key>, children:seq<Child>)
 datatype Sector =
       Superblock(firstCold:LBA, warm:set<LBA>, virgin:LBA)
     | ColdFreeList(next:LBA)
-    | Node(parent:LBA, pivots:seq<Key>, children:seq<Child>)
+    | NodeSector(node:Node)
 
 } // module TreeDisk
 
@@ -30,15 +30,17 @@ function Last<T>(s:seq<T>) : T  // TODO move to library
 }
 
 type LBA = TreeDisk.LBA
+type Child = TreeDisk.Child
 type Sector = TreeDisk.Sector
+type Node = TreeDisk.Node
 
-// CRead == a "cached read"
-datatype CRead = CRead(lba:LBA, sector:Sector)
+// NRead == a "cached read" of a node
+datatype NRead = NRead(lba:LBA, node:Node)
 
 datatype Constants = Constants(disk:TreeDisk.Constants)
 datatype Variables = Variables(
     disk:TreeDisk.Variables,
-    cache:map<LBA, TreeDisk.Sector>,
+    cache:map<LBA, Sector>,
 
     // We don't REALLY need to track uncommittedFreeListHead in the spec; we COULD
     // exists a cache-observable chain into existence whenever we need it.
@@ -53,26 +55,46 @@ function ROOT_LBA() : LBA { 1 }
 // 0 is a fine null LBA pointer, since we never need to point at the superblock.
 function NULLPTR() : LBA { 0 }
 
+predicate WFNode(node:Node) {
+    |node.pivots| == |node.children| - 1
+}
+
 predicate Init(k:Constants, s:Variables)
 {
     && TreeDisk.Init(k.disk, s.disk)
     && TreeDisk.Peek(k.disk, s.disk, SUPERBLOCK_LBA(), TreeDisk.Superblock(NULLPTR(), {}, 2))
-    && TreeDisk.Peek(k.disk, s.disk, ROOT_LBA(), TreeDisk.Node(NULLPTR(), [], [TreeDisk.Empty]))
+    && TreeDisk.Peek(k.disk, s.disk, ROOT_LBA(),
+        TreeDisk.NodeSector(TreeDisk.Node(NULLPTR(), [], [TreeDisk.Empty])))
     && s.cache.Keys == {}
 }
 
 // State predicate: we can read lba->sector out of the in-memory cache
-predicate CachedRead(k:Constants, s:Variables, cread:CRead)
+predicate CachedSectorRead(k:Constants, s:Variables, lba:LBA, sector:Sector)
 {
-    && cread.lba in s.cache
-    && s.cache[cread.lba] == cread.sector
+    && lba in s.cache
+    && s.cache[lba] == sector
+}
+
+predicate CachedNodeRead(k:Constants, s:Variables, nread:NRead)
+{
+    && CachedSectorRead(k, s, nread.lba, TreeDisk.NodeSector(nread.node))
+    // We toss WFNode in here to keep other expressions tidy; as with any WF, this can
+    // create a liveness problem (can't read that disk sector with a malformed node).
+    // Even if we don't prove liveness, we can mitigate that concern by including a
+    // WF invariant.
+    && WFNode(nread.node)
 }
 
 // Partial action: Write a sector out, through the cache
-predicate WriteThrough(k:Constants, s:Variables, s':Variables, lba:LBA, sector:Sector)
+predicate WriteThroughSector(k:Constants, s:Variables, s':Variables, lba:LBA, sector:Sector)
 {
     && TreeDisk.Write(k.disk, s.disk, s'.disk, lba, sector)
     && s'.cache == s.cache[lba := sector]
+}
+
+predicate WriteThroughNode(k:Constants, s:Variables, s':Variables, lba:LBA, node:Node)
+{
+    WriteThroughSector(k, s, s', lba, TreeDisk.NodeSector(node))
 }
 
 // Bring a sector into the cache
@@ -96,7 +118,7 @@ predicate CacheEvictAction(k:Constants, s:Variables, s':Variables, lba:LBA)
     && s'.cache == MapRemove(s.cache, lba)
 }
 
-predicate NodeDisownsChild(parent:Sector, childLba:LBA)
+predicate NodeDisownsChild(parent:Node, childLba:LBA)
 {
     forall idx :: 0<=idx<|parent.children| ==> parent.children[idx] != TreeDisk.Pointer(childLba)
 }
@@ -115,20 +137,62 @@ predicate RangeContains(range:Range, key:Key)
 }
 
 datatype PathElt = PathElt(
-    cread:CRead, // this node
-    idx:int,     // index of path[i+1].cread.lba in children[] 
+    nread:NRead, // this node
+    idx:int,     // index of path[i+1].nread.lba in children[] 
     range:Range  // bounds for keys at this node
     )    
 
+predicate ValidChildIndex(node:Node, idx:int)
+{
+     0 <= idx < |node.children|
+}
+
 // If all of node's keys are bounded by nodeRange, then
 // the keys in the i'th children of node are bounded by range.
-function RangeBoundForChildIdx(node:Sector, nodeRange:Range, i:int) : (range:Range)
-    requires node.Node?
-    requires 0<=i<|node.children|
+function RangeBoundForChildIdx(node:Node, nodeRange:Range, i:int) : (range:Range)
+    requires WFNode(node)
+    requires ValidChildIndex(node, i)
 {
     Range(
         if i==0 then nodeRange.loinc else node.pivots[i-1],
         if i==|node.children|-1 then nodeRange.hiexc else node.pivots[i])
+}
+
+// All of the nodes in the path are as read out of the cache (we didn't just make them up).
+predicate PathIsCached(k:Constants, s:Variables, path:seq<PathElt>)
+{
+    forall i :: 0<=i<|path| ==> CachedNodeRead(k, s, path[i].nread)
+}
+
+predicate PathHasValidChildIndices(k:Constants, s:Variables, path:seq<PathElt>)
+{
+    forall i :: 0<=i<|path| ==> (
+        var pElt := path[i];
+        && ValidChildIndex(pElt.nread.node, pElt.idx)
+    )
+}
+
+// All of the node pairs in the path reflect a parent-child link given at the
+// path element's index in the parent.
+predicate PathLinksChildren(k:Constants, s:Variables, path:seq<PathElt>)
+    requires PathHasValidChildIndices(k, s, path)
+{
+    forall i :: 0<=i<|path|-1 ==> (
+        var pElt := path[i];
+        && pElt.nread.node.children[pElt.idx] == TreeDisk.Pointer(path[i+1].nread.lba)
+    )
+}
+
+// The ranges noted in the pathElts reflect the ranges imposed by the parent's
+// range and pivots
+predicate PathNestsRanges(k:Constants, s:Variables, path:seq<PathElt>)
+    requires PathIsCached(k, s, path)
+    requires PathHasValidChildIndices(k, s, path)
+{
+    forall i :: 0<=i<|path|-1 ==> (
+        var pElt := path[i];
+        assert ValidChildIndex(pElt.nread.node, pElt.idx);
+        && RangeBoundForChildIdx(pElt.nread.node, pElt.range, pElt.idx) == path[i+1].range)
 }
 
 // True if every Node in path is live (committed) tree data.
@@ -136,130 +200,123 @@ function RangeBoundForChildIdx(node:Sector, nodeRange:Range, i:int) : (range:Ran
 predicate CachedPathRead(k:Constants, s:Variables, path:seq<PathElt>)
 {
     && 0<|path|
-    && path[0].cread.lba == ROOT_LBA()
-    && forall i :: 0<=i<|path| ==> (
-        var pElt := path[i];
-        && CachedRead(k, s, pElt.cread)
-        && i<|path|-1 ==> (
-            && pElt.cread.sector.Node?   // TODO factor Node out of Sector
-            && 0 <= pElt.idx < |pElt.cread.sector.children|
-            && pElt.cread.sector.children[i] == TreeDisk.Pointer(path[i+1].cread.lba)
-            )
-        // Ranges next correctly
-        && RangeBoundForChildIdx(pElt.cread.sector, pElt.range, pElt.idx) == path[i+1].range
-        )
-
-    && (forall i :: 0<=i<|path|-1 ==> !NodeDisownsChild(path[i].cread.sector, path[i+1].cread.lba))
+    && path[0].nread.lba == ROOT_LBA()
+    && PathIsCached(k, s, path)
+    && PathHasValidChildIndices(k, s, path)
+    && PathLinksChildren(k, s, path)
+    && PathNestsRanges(k, s, path)
 }
 
-predicate NodeIsLive(k:Constants, s:Variables, node:CRead)
+predicate NodeIsLive(k:Constants, s:Variables, node:NRead)
 {
     exists path:seq<PathElt> :: (
         && CachedPathRead(k, s, path)
-        && Last(path).cread == node
+        && Last(path).nread == node
     )
 }
 
-predicate NodeIsCold(k:Constants, s:Variables, nodeRead:CRead)
+predicate NodeIsCold(k:Constants, s:Variables, lba:LBA, sector:Sector)
 {
-    && CachedRead(k, s, nodeRead)
-    && !nodeRead.sector.Node?
+    && CachedSectorRead(k, s, lba, sector)
+    && !sector.NodeSector?
 }
 
 // childLba is a Node that's not connected to the live tree.
 // (This test isn't complete; a node connected to a disconnected ancestor will not satisfy
 // this predicate. But it lets us always reuse a frontier of nodes.)
-predicate NodeDisconnected(k:Constants, s:Variables, childRead:CRead)
+predicate NodeDisconnected(k:Constants, s:Variables, childRead:NRead)
 {
-    exists parentRead:CRead :: (
+    exists parentRead:NRead :: (
         // Child thinks it belongs to parent
-        && CachedRead(k, s, childRead)
-        && childRead.sector.Node?
-        && childRead.sector.parent == parentRead.lba
+        && CachedNodeRead(k, s, childRead)
+        && childRead.node.parent == parentRead.lba
         && (
-            || (NodeIsLive(k, s, parentRead) && NodeDisownsChild(parentRead.sector, childRead.lba))
-            || NodeIsCold(k, s, parentRead)
+            || (NodeIsLive(k, s, parentRead) && NodeDisownsChild(parentRead.node, childRead.lba))
+            || NodeIsCold(k, s, parentRead.lba, TreeDisk.NodeSector(parentRead.node))
            )
     )
 }
 
 
-predicate CanAllocate(k:Constants, s:Variables, childRead:CRead)
+predicate CanAllocate(k:Constants, s:Variables, childRead:NRead)
 {
     || NodeDisconnected(k, s, childRead)
-    || NodeIsCold(k, s, childRead)
+    || NodeIsCold(k, s, childRead.lba, TreeDisk.NodeSector(childRead.node))
 }
 
-function ChildNodeForParentIdx(parentRead:CRead, i:int) : Sector
-    requires 0<=i<|parentRead.sector.children|
+function ChildNodeForParentIdx(parentRead:NRead, i:int) : Node
+    requires 0<=i<|parentRead.node.children|
 {
-    TreeDisk.Node(parentRead.lba, [], [parentRead.sector.children[i]])
+    TreeDisk.Node(parentRead.lba, [], [parentRead.node.children[i]])
 }
 
 // Create a new uncommitted child that thinks it belongs to parent, ready to replace children[i].
 // We should check that this ensures KnowPrepared(s', ...)
 // (Or we could WRITE this as KnowPrepared(k, s', ...) -- but that's harder to
 // see as an implementation?)
-predicate PrepareGrowAction(k:Constants, s:Variables, s':Variables, parentRead:CRead, i:int, childRead:CRead)
+predicate PrepareGrowAction(k:Constants, s:Variables, s':Variables, parentRead:NRead, i:int, childRead:NRead)
 {
-    && CachedRead(k, s, parentRead)
-    && 0<=i<|parentRead.sector.children|
+    && CachedNodeRead(k, s, parentRead)
+    && 0<=i<|parentRead.node.children|
     && CanAllocate(k, s, childRead)
-    && WriteThrough(k, s, s', childRead.lba, ChildNodeForParentIdx(parentRead, i))
+    && WriteThroughNode(k, s, s', childRead.lba, ChildNodeForParentIdx(parentRead, i))
 }
 
-predicate KnowPrepared(k:Constants, s:Variables, parentRead:CRead, i:int, childRead:CRead)
+predicate KnowPrepared(k:Constants, s:Variables, parentRead:NRead, i:int, childRead:NRead)
 {
-    && CachedRead(k, s, parentRead)
-    && 0<=i<|parentRead.sector.children|
-    && CachedRead(k, s, childRead)
+    && CachedNodeRead(k, s, parentRead)
+    && 0<=i<|parentRead.node.children|
+    && CachedNodeRead(k, s, childRead)
     // Do we need to ensure child isn't hot? Well, obviously not if its parent pointer points
     // to parent, and there's a parent-child consistency invariant.
-    && childRead.sector == ChildNodeForParentIdx(parentRead, i)
+    && childRead.node == ChildNodeForParentIdx(parentRead, i)
 }
 
-function SectorUpdateChild(parent:Sector, i:int, child:TreeDisk.Child) : Sector
-    requires parent.Node?
+function SectorUpdateChild(parent:Node, i:int, child:Child) : Node
+    requires 0<=i<|parent.children|
 {
     TreeDisk.Node(parent.parent, parent.pivots,
         parent.children[..i] + [child] + parent.children[i+1..])
 }
 
-predicate CommitGrowAction(k:Constants, s:Variables, s':Variables, parentRead:CRead, i:int, childRead:CRead)
+predicate CommitGrowAction(k:Constants, s:Variables, s':Variables, parentRead:NRead, i:int, childRead:NRead)
 {
     && KnowPrepared(k, s, parentRead, i, childRead)
-    && WriteThrough(k, s, s', parentRead.lba, SectorUpdateChild(parentRead.sector, i,
+    && WriteThroughNode(k, s, s', parentRead.lba, SectorUpdateChild(parentRead.node, i,
         TreeDisk.Pointer(childRead.lba)))
 }
 
-predicate ContractNodeAction(k:Constants, s:Variables, s':Variables, parentRead:CRead, i:int, childRead:CRead)
+predicate ContractNodeAction(k:Constants, s:Variables, s':Variables, parentRead:NRead, i:int, childRead:NRead)
 {
     && NodeIsLive(k, s, parentRead)
-    && CachedRead(k, s, childRead)
-    && childRead.sector.Node?
-    && childRead.sector.pivots == []    // child has one child, which can take its place in parent.
-    && WriteThrough(k, s, s', parentRead.lba,
-        SectorUpdateChild(parentRead.sector, i, childRead.sector.children[0]))
+    && CachedNodeRead(k, s, childRead)
+    && childRead.node.pivots == []    // child has one child, which can take its place in parent.
+    && 0<=i<|parentRead.node.children|
+    && WriteThroughNode(k, s, s', parentRead.lba,
+        SectorUpdateChild(parentRead.node, i, childRead.node.children[0]))
     // This write causes child to become free-by-unreachable. So child must be in committed warm set.
 }
 
 // There's a live path leading to node, and it supports range as a bound for node.
-predicate LivePathBoundsChild(k:Constants, s:Variables, node:CRead, idx:int, range:Range)
+predicate LivePathBoundsChild(k:Constants, s:Variables, node:NRead, idx:int, range:Range)
 {
     exists path : seq<PathElt> :: (
         && CachedPathRead(k, s, path)
-        && Last(path).cread == node
+        && Last(path).nread == node
         && Last(path).idx == idx
-        && RangeBoundForChildIdx(Last(path).cread.sector, Last(path).range, Last(path).idx) == range
+        && PathHasValidChildIndices(k, s, path)
+        && RangeBoundForChildIdx(Last(path).nread.node, Last(path).range, Last(path).idx) == range
     )
 }
 
-predicate QueryAction(k:Constants, s:Variables, s':Variables, nodeRead:CRead, idx:int, range:Range, datum:Datum)
+predicate QueryAction(k:Constants, s:Variables, s':Variables, nodeRead:NRead, idx:int, range:Range, datum:Datum)
 {
-    var childRange := RangeBoundForChildIdx(nodeRead.sector, range, idx);
+    && WFNode(nodeRead.node)
+    && ValidChildIndex(nodeRead.node, idx)
+    && var childRange := RangeBoundForChildIdx(nodeRead.node, range, idx);
     && LivePathBoundsChild(k, s, nodeRead, idx, range)
     && RangeContains(range, datum.key)
-    && var child := nodeRead.sector.children[idx]; (
+    && var child := nodeRead.node.children[idx]; (
         || (child.Value? && child.datum == datum)
         || (child.Value? && child.datum.key != datum.key && datum.value == EmptyValue())
         || (child.Empty? && datum.value == EmptyValue())
@@ -269,8 +326,9 @@ predicate QueryAction(k:Constants, s:Variables, s':Variables, nodeRead:CRead, id
 // Insert newPivot at idx (shifting old pivot[idx] to the right).
 // Replace child[idx] with newChildren.
 // In practice, |newChildren|=2, and one of its elements is the old child[idx].
-function SectorInsertChild(parent:Sector, idx:int, newPivot:Key, newChildren:seq<TreeDisk.Child>) : Sector
-    requires parent.Node?
+function SectorInsertChild(parent:Node, idx:int, newPivot:Key, newChildren:seq<Child>) : Node
+    requires WFNode(parent)
+    requires 0<=idx<|parent.children|
 {
     TreeDisk.Node(parent.parent,
         parent.pivots[..idx] + [newPivot] + parent.pivots[idx..],
@@ -279,53 +337,56 @@ function SectorInsertChild(parent:Sector, idx:int, newPivot:Key, newChildren:seq
 // newDatum.key is absent from the tree; insert it near a neighboring pivot
 predicate InsertAction(k:Constants, s:Variables, s':Variables, newDatum:Datum)
 {
-    exists nodeRead:CRead, range:Range, idx:int :: (
+    exists nodeRead:NRead, range:Range, idx:int :: (
         // Find a leaf that we can split.
-        var childRange := RangeBoundForChildIdx(nodeRead.sector, range, idx);
-        var extantChild := nodeRead.sector.children[idx];
+        && WFNode(nodeRead.node)
+        && ValidChildIndex(nodeRead.node, idx)
+        && var childRange := RangeBoundForChildIdx(nodeRead.node, range, idx);
+        && var extantChild := nodeRead.node.children[idx];
         && LivePathBoundsChild(k, s, nodeRead, idx, range)
         && RangeContains(range, newDatum.key)
         && !extantChild.Pointer?
         // This is an insert, not a replace
         && if extantChild.Empty? || newDatum.key == extantChild.datum.key
                 // Replace an empty or same-key datum in place
-            then WriteThrough(k, s, s', nodeRead.lba,
-                SectorUpdateChild(nodeRead.sector, idx, TreeDisk.Value(newDatum)))
+            then WriteThroughNode(k, s, s', nodeRead.lba,
+                SectorUpdateChild(nodeRead.node, idx, TreeDisk.Value(newDatum)))
             else if KeyLe(newDatum.key, extantChild.datum.key)
                 // New datum goes to the left, so we'll split a pivot to the right with the old key
-            then WriteThrough(k, s, s', nodeRead.lba,
-                SectorInsertChild(nodeRead.sector, idx, extantChild.datum.key, [TreeDisk.Value(newDatum), extantChild]))
+            then WriteThroughNode(k, s, s', nodeRead.lba,
+                SectorInsertChild(nodeRead.node, idx, extantChild.datum.key, [TreeDisk.Value(newDatum), extantChild]))
                 // New datum goes to the right, so we'll split a pivot with the new key
-            else WriteThrough(k, s, s', nodeRead.lba,
-                SectorInsertChild(nodeRead.sector, idx, newDatum.key, [extantChild, TreeDisk.Value(newDatum)]))
+            else WriteThroughNode(k, s, s', nodeRead.lba,
+                SectorInsertChild(nodeRead.node, idx, newDatum.key, [extantChild, TreeDisk.Value(newDatum)]))
     )
 }
 
-predicate DeleteAction(k:Constants, s:Variables, s':Variables, newDatum:Datum, nodeRead:CRead, idx:int, range:Range)
+predicate DeleteAction(k:Constants, s:Variables, s':Variables, newDatum:Datum, nodeRead:NRead, idx:int, range:Range)
 {
     && LivePathBoundsChild(k, s, nodeRead, idx, range)  // don't actually care about range
-    && nodeRead.sector.children[idx] == TreeDisk.Value(newDatum)
-    // Replace child with Empty. TODO background clean up of empty children where feasible.
-    // (Contract cleans up small children.)
-    && WriteThrough(k, s, s', nodeRead.lba,
-        SectorUpdateChild(nodeRead.sector, idx, TreeDisk.Empty))
+    && nodeRead.node.children[idx] == TreeDisk.Value(newDatum)
+    // Replace child with Empty.
+    // TODO background clean up of empty children within a node where feasible.
+    // (Contract action already cleans up small children.)
+    && WriteThroughNode(k, s, s', nodeRead.lba,
+        SectorUpdateChild(nodeRead.node, idx, TreeDisk.Empty))
 }
 
 // Move an unreachable node onto an uncommitted free list
-predicate MoveToFreeListAction(k:Constants, s:Variables, s':Variables, lba:LBA, childRead:CRead)
+predicate MoveToFreeListAction(k:Constants, s:Variables, s':Variables, lba:LBA, childRead:NRead)
 {
-    && CachedRead(k, s, childRead)
+    && CachedNodeRead(k, s, childRead)
     && NodeDisconnected(k, s, childRead)
-    && WriteThrough(k, s, s', lba, TreeDisk.ColdFreeList(s.uncommittedFreeListHead))
+    && WriteThroughSector(k, s, s', lba, TreeDisk.ColdFreeList(s.uncommittedFreeListHead))
     && s'.uncommittedFreeListHead == lba
 }
 
-predicate CommitFreeListAction(k:Constants, s:Variables, s':Variables, lba:LBA, super:CRead)
+predicate CommitFreeListAction(k:Constants, s:Variables, s':Variables, super:Sector)
 {
-    && super.lba == SUPERBLOCK_LBA()
-    && CachedRead(k, s, super)
-    && WriteThrough(k, s, s', super.lba,
-        TreeDisk.Superblock(s.uncommittedFreeListHead, super.sector.warm, super.sector.virgin))
+    && CachedSectorRead(k, s, SUPERBLOCK_LBA(), super)
+    && super.Superblock?
+    && WriteThroughSector(k, s, s', SUPERBLOCK_LBA(),
+        TreeDisk.Superblock(s.uncommittedFreeListHead, super.warm, super.virgin))
 }
 
 
